Split prf_{sem,bounds_check} into separate files.
Using a nested module resulted in weird behaviour wrt. the type class in
Context.

theories/approxis/examples/prf.v
@@ -14,22 +14,22 @@ Class PRF :=
   ; rand_output : val
   }.
 
-Section random_function.
-  Context `{PRF}.
+(* An idealised random function family. *)
+Definition random_function (card_output : nat) : val :=
+  λ: "_key",
+    (* Create a reference to a functional map *)
+    let: "mapref" := init_map #() in
+    λ: "x",
+      match: get "mapref" "x" with
+      | SOME "y" => "y"
+      | NONE =>
+          let: "y" := (rand #card_output) in
+          set "mapref" "x" "y";;
+          "y"
+      end.
 
-  (* An idealised random function family. *)
-  Definition random_function : val :=
-    λ: "_key",
-      (* Create a reference to a functional map *)
-      let: "mapref" := init_map #() in
-      λ: "x",
-        match: get "mapref" "x" with
-        | SOME "y" => "y"
-        | NONE =>
-            let: "y" := (rand #card_output) in
-            set "mapref" "x" "y";;
-            "y"
-        end.
+Section lrel.
+  Context `{PRF}.
 
   Definition lrel_key {Σ} : lrel Σ := lrel_int_bounded 0 card_key.
   Definition lrel_input {Σ} : lrel Σ := lrel_int_bounded 0 card_input.
@@ -39,7 +39,7 @@ Section random_function.
 
   Definition lrel_PRF_Adv `{!approxisRGS Σ} := ((lrel_input → (lrel_option lrel_output)) → lrel_bool)%lrel.
 
-End random_function.
+End lrel.
 
 
 Module LR_prf.
@@ -106,11 +106,10 @@ End LR_prf.
 Export LR_prf.
 
 Section random_function.
-  Context `{PRF}.
 
-  Fact random_function_sem_typed `{!approxisRGS Σ} A :
-    ⊢ REL random_function
-        << random_function : A → lrel_input → lrel_output.
+  Fact random_function_sem_typed `{!approxisRGS Σ} `{PRF} A :
+    ⊢ REL (random_function card_output)
+        << (random_function card_output) : A → lrel_input → lrel_output.
   Proof with (rel_pures_l ; rel_pures_r).
     rel_arrow_val ; iIntros (??) "_".
     rewrite /random_function...
@@ -169,71 +168,11 @@ Section random_function.
       }
       rel_vals. Unshelve. all: apply _.
   Qed.
-End random_function.
-
-(** PRF security definitions using the variant of q_calls with explicit bounds
-    checks in the code. **)
-Module bound_checks.
-
-  Context `{PRF}.
-
-  (* Variable Key Input Output : nat.
-
-     Let keygen PRF_scheme : expr := Fst PRF_scheme.
-     Let prf PRF_scheme : expr := Fst (Snd PRF_scheme).
-     Let rand_output PRF_scheme : expr := Snd (Snd PRF_scheme). *)
-
-  Let q_calls := q_calls card_input.
-
-  Definition PRF_real_rand : val :=
-    λ:"b" "adv" "PRF_scheme" "Q",
-      let: "key" := keygen "PRF_scheme" #() in
-      let: "prf_key_b" :=
-        if: "b" then
-          prf "PRF_scheme" "key"
-        else
-          random_function "key" in
-      let: "oracle" := q_calls "Q" "prf_key_b" in
-      let: "b'" := "adv" "oracle" in
-      "b'".
-
-  Definition wPRF : val :=
-    λ:"b" "PRF_scheme" "Q",
-      let: "key" := keygen "PRF_scheme" #() in
-      let: "prf_key_b" :=
-        if: "b" then
-          prf "PRF_scheme" "key"
-        else
-          random_function "key" in
-      let: "res" := ref list_nil in
-      letrec: "loop" "i" :=
-          if: "i" = #0 then #() else
-            let: "x" := rand #card_input in
-            let: "y" := "prf_key_b" "x" in
-            "res" <- list_cons ("x", "y") (!"res") ;;
-            "loop" ("i" - #1)
-      in
-      ("loop" "Q") ;;
-      ! "res".
-
-  (* Rosulek, Def. 6.1 (PRF security) *)
-  (* NB: Rosulek samples the key from {0,1}^λ, we sample it from [0,card_key]. *)
-  Definition PRF_real : val :=
-    λ:"PRF_scheme" "Q",
-      let: "k" := keygen "PRF_scheme" #() in
-      let: "lookup" := prf "PRF_scheme" "k" in
-      let: "oracle" := q_calls "Q" "lookup" in
-      "oracle".
-
-  Definition PRF_rand : val :=
-    λ:"PRF_scheme" "Q",
-      let: "lookup" := random_function #() in
-      let: "oracle" := q_calls "Q" "lookup" in
-      "oracle".
 
   Section spec_ideal.
 
     Context `{!approxisGS Σ}.
+    Variable (card_output : nat).
 
     (* To hash a value v, we check whether it is in the map (i.e. it has been previously hashed).
      If it has we return the saved hash value, otherwise we draw a hash value and save it in the map *)
@@ -272,7 +211,7 @@ Module bound_checks.
 
     Lemma wp_random_function E :
       {{{ True }}}
-        random_function #() @ E
+        random_function card_output #() @ E
         {{{ f, RET f; is_random_function f ∅ }}}.
     Proof.
       rewrite /random_function.
@@ -284,132 +223,7 @@ Module bound_checks.
     Qed.
 
     Lemma spec_random_function E K:
-      ⤇ fill K (random_function #()) -∗
-      spec_update E (∃ (f:val), ⤇ fill K f ∗ is_srandom_function f ∅).
-    Proof.
-      rewrite /random_function.
-      iIntros "Hspec".
-      tp_pures.
-      tp_bind (init_map _).
-      iMod (spec_init_map with "[$]") as "(%&?&?)".
-      simpl. tp_pures.
-      iApply spec_update_ret.
-      by iFrame.
-    Qed.
-
-    Lemma wp_random_function_prev E f m (n : nat) (b : Z) :
-      m !! n = Some b →
-      {{{ is_random_function f m }}}
-        f #n @ E
-        {{{ RET #b; is_random_function f m }}}.
-    Proof.
-      iIntros (Hlookup Φ) "Hhash HΦ".
-      iDestruct "Hhash" as (hm ->) "H".
-      rewrite /compute_rf_specialized.
-      wp_pures.
-      wp_apply (wp_get with "[$]").
-      iIntros (vret) "(Hhash&->)".
-      rewrite lookup_fmap Hlookup /=. wp_pures. iModIntro. iApply "HΦ".
-      iExists _. eauto.
-    Qed.
-
-    
-    Lemma spec_random_function_prev E f m (n : nat) (b : Z) K:
-      m !! n = Some b →
-      is_srandom_function f m -∗
-      ⤇ fill K (f #n) -∗
-      spec_update E (⤇ fill K #b ∗ is_srandom_function f m).
-    Proof.
-      iIntros (Hlookup) "Hhash Hspec".
-      iDestruct "Hhash" as (hm ->) "H".
-      rewrite /compute_rf_specialized.
-      tp_pures.
-      tp_bind (get _ _).
-      iMod (spec_get with "[$][$]") as "(?&?)".
-      simpl. 
-      rewrite lookup_fmap Hlookup /=. tp_pures. iModIntro.
-      iFrame. auto.
-    Qed.
-    
-  End spec_ideal.
-
-End bound_checks.
-
-(** PRF security definitions using the variant of q_calls using semantic typing
-    instead of bounds checks. **)
-Module sem.
-
-  Context `{PRF}.
-
-  Let q_calls := q_calls_poly.
-
-  Definition PRF_real : val :=
-    λ:"Q",
-      let: "k" := keygen #() in
-      let: "lookup" := prf "k" in
-      let: "oracle" := q_calls_poly #() #() "Q" "lookup" in
-      "oracle".
-
-  Definition PRF_rand : val :=
-    λ:"PRF_scheme" "Q",
-      let: "lookup" := random_function #() in
-      let: "oracle" := q_calls_poly #() #() "Q" "lookup" in
-      "oracle".
-
-  Section spec_ideal.
-
-    Context `{!approxisGS Σ}.
-
-    (* To hash a value v, we check whether it is in the map (i.e. it has been previously hashed).
-     If it has we return the saved hash value, otherwise we draw a hash value and save it in the map *)
-    Definition compute_rf_specialized hm : val :=
-      λ: "x",
-        match: get hm "x" with
-        | SOME "y" => "y"
-        | NONE =>
-            let: "y" := (rand #card_output) in
-            set hm "x" "y";;
-            "y"
-        end.
-    Definition compute_rf : val :=
-      λ: "mapref" "x",
-        match: get "mapref" "x" with
-        | SOME "y" => "y"
-        | NONE =>
-            let: "y" := (rand #card_output) in
-            set "mapref" "x" "y";;
-            "y"
-        end.
-
-    Definition is_random_function f m : iProp Σ :=
-      ∃ (mapref : loc), ⌜ f = compute_rf_specialized #mapref ⌝ ∗ map_list mapref ((λ b, LitV (LitInt b)) <$> m).
-
-    Definition is_srandom_function f m : iProp Σ :=
-      ∃ (mapref : loc), ⌜ f = compute_rf_specialized #mapref ⌝ ∗ map_slist mapref ((λ b, LitV (LitInt b)) <$> m).
-
-    #[global] Instance timeless_is_random_function f m :
-      Timeless (is_random_function f m).
-    Proof. apply _. Qed.
-
-    #[global] Instance timeless_is_srandom_function f m :
-      Timeless (is_srandom_function f m).
-    Proof. apply _. Qed.
-
-    Lemma wp_random_function E :
-      {{{ True }}}
-        random_function #() @ E
-        {{{ f, RET f; is_random_function f ∅ }}}.
-    Proof.
-      rewrite /random_function.
-      iIntros (Φ) "_ HΦ".
-      wp_pures.
-      wp_apply (wp_init_map with "[//]").
-      iIntros (?) "Hm". wp_pures.
-      iApply "HΦ". iExists _. rewrite fmap_empty. iFrame. eauto.
-    Qed.
-
-    Lemma spec_random_function E K:
-      ⤇ fill K (random_function #()) -∗
+      ⤇ fill K (random_function card_output #()) -∗
       spec_update E (∃ (f:val), ⤇ fill K f ∗ is_srandom_function f ∅).
     Proof.
       rewrite /random_function.
@@ -458,4 +272,4 @@ Module sem.
 
   End spec_ideal.
 
-End sem.
+End random_function.
